\documentclass[ClusteringConnectionsMAIN.tex]{subfiles}




\begin{document}
	

\prob{2.31}  Starting with $\Hent{ X \mid g \left( Y \right) } = \Hent{X \mid Y}$, we multiply both sides by $-1$ before adding $\Hent{X}$ to both sides to obtain

\begin{align}  \label{c2p31eq1}
\Hent{ X \mid g \left( Y \right) } &= \Hent{X \mid Y}   \notag \\
\Hent{X} - \Hent{ X \mid g \left( Y \right) } &= \Hent{X} - \Hent{X \mid Y} \notag  \\
\I{X; g \left( X \right) } &= \I{X; Y}  \tag{2.31-1}
\end{align}

by noting the definition of mutual information.  The expression in \ref{c2p31eq1} implies that in order for $\Hent{ X \mid g \left( Y \right) } = \Hent{X \mid Y}$ to be true, $\I{X; g \left( X \right) } = \I{X; Y}$ must hold.






































\end{document}