\documentclass[ClusteringConnectionsMAIN.tex]{subfiles}




\begin{document}
	

\prob{2.11 a}  Starting with

\begin{align} \label{c2p11eq1}
\rho &= 1 - \frac{ \Hent{X_2 \mid X_1} }{ \Hent{X_1} }  \tag{2.11-1}
\end{align}

We obtain a common denominator and note that, since $X_1$ and $X_2$ are identically distributed, $\Hent{X_1} = \Hent{X_2}$ to yield the result

\begin{align} 
\rho &= 1 - \frac{ \Hent{X_2 \mid X_1} }{ \Hent{X_1} }   \notag \\
&= \frac{ \Hent{X_1} - \Hent{X_2 \mid X_1} }{ \Hent{X_1} }  \notag \\
&= \frac{ \Hent{X_2} - \Hent{X_2 \mid X_1} }{ \Hent{X_1} }  \notag
\end{align}

Now, since $\I{X_1; X_2} = \Hent{X_1} - \Hent{X_1 \mid X_2} = \Hent{X_2} - \Hent{X_2 \mid X_1}$, the previous result finally becomes

\begin{align} \label{c2p11eq2}
\rho &= \frac{ \Hent{X_2} - \Hent{X_2 \mid X_1} }{ \Hent{X_1} }  \notag \\
&= \frac{ \I{X_2; X_1 } }{ \Hent{X_1} } = \boxed{ \frac{ \I{X_1; X_2} }{ \Hent{X_1} } }   \tag{2.11-2}
\end{align}





































\end{document}